theories/logrel/logrel.v
@@ -44,14 +44,14 @@ Section logrel.
      while the sender needs full to reclaim, we let i always own half and only pass the otner half around with VMProp*)
   (* [TODO] relation to [pagetable_entries_excl_owned] *)
   Definition transaction_pagetable_entries_owned (trans: gmap Addr transaction) : iProp Σ:=
-    big_sepFM trans (λ kv, kv.2.1.1.1.1.1 = i ∧ kv.2.1.2 ≠ Donation) (λ k v, k -{1/2}>t v.1 ∗ pgt v.1.1.2 1 v.1.1.1.1.1 (bool_decide (v.1.2 ≠ Sharing)))%I.
+    big_sepFM trans (λ kv, kv.2.1.1.1.1 = i ∧ kv.2.1.2 ≠ Donation) (λ k v, k -{1/2}>t v.1 ∗ pgt v.1.1.2 1 v.1.1.1.1 (bool_decide (v.1.2 ≠ Sharing)))%I.
 
    (* [transaction_pagetable_entries_transferred] : For donation, the half of transaction entries that are kept by sender in case
       of sharing and lending are also be passed around between the sender and the receiver, as retrieval in this case also requires
       full entries.
       Pagetable entries are transferred along as both sender and receiver could be the exclusive owner of those pages. *)
   Definition transaction_pagetable_entries_transferred (trans: gmap Addr transaction) : iProp Σ:=
-    big_sepFM trans (λ kv, kv.2.1.2 = Donation ∧ (kv.2.1.1.1.2 = i ∨ kv.2.1.1.1.1.1 = i)) (λ k v, k -{1/2}>t v.1 ∗ pgt v.1.1.2 1 v.1.1.1.1.1 true)%I.
+    big_sepFM trans (λ kv, kv.2.1.2 = Donation ∧ (kv.2.1.1.1.2 = i ∨ kv.2.1.1.1.1 = i)) (λ k v, k -{1/2}>t v.1 ∗ pgt v.1.1.2 1 v.1.1.1.1 true)%I.
 
   (* [retrieval entries]: half of all retrieval entries of i-related transactions are required.
      For transactions where i is the sender, we need the corresponding retrieval entries to check if it is allowed for i to reclaim,
@@ -59,8 +59,8 @@ Section logrel.
   (* There are also some cases when we need the second half, as in those cases we may update/remove the retrival state *)
   (* XXX: How to relate retrieval and transaction entries? Using option(frac_agree transaction,option bool)? or is it unnecessary? *)
   Definition retrieval_entries_transferred(trans: gmap Addr transaction) : iProp Σ:=
-    (big_sepFM trans (λ kv, kv.2.1.1.1.2 = i ∨ kv.2.1.1.1.1.1 = i) (λ k v, k -{1/2}>re v.2 )%I) ∗
-    (big_sepFM trans (λ kv, (kv.2.1.1.1.1.1 = i ∨ kv.2.1.1.1.2 = i) ∧ kv.2.2 = false) (λ k v, k -{1/2}>re v.2)%I).
+    (big_sepFM trans (λ kv, kv.2.1.1.1.2 = i ∨ kv.2.1.1.1.1 = i) (λ k v, k -{1/2}>re v.2 )%I) ∗
+    (big_sepFM trans (λ kv, (kv.2.1.1.1.1 = i ∨ kv.2.1.1.1.2 = i) ∧ kv.2.2 = false) (λ k v, k -{1/2}>re v.2)%I).
 
   (* [TODO] *)
   Definition retrieval_entries_owned(trans: gmap Addr transaction) : iProp Σ:=
@@ -69,7 +69,7 @@ Section logrel.
   (* [memory_transferred]: some memory points-to predicates are transferred by VMProp.
      the memory is the memory of pages associated with a transaction and i has or may have access to. *)
   Definition trans_memory_in_trans (trans : gmap Word transaction) :=
-    filter (λ kv, (kv.2.1.1.1.1.1 = i ∧ ¬(kv.2.2 = true ∧ kv.2.1.2 = Lending)) ∨ kv.2.1.1.1.2 = i) trans.
+    filter (λ kv, (kv.2.1.1.1.1 = i ∧ ¬(kv.2.2 = true ∧ kv.2.1.2 = Lending)) ∨ kv.2.1.1.1.2 = i) trans.
   Definition memory_transferred (trans : gmap Word transaction) (mem: mem) :=
    memory_pages (pages_in_trans (trans_memory_in_trans trans)) mem.
 
