theories/rules/mem_retrieve.v
@@ -8,7 +8,7 @@ Section retrieve.
 Context `{hypparams: HypervisorParameters}.
 Context `{vmG: !gen_VMG Σ}.
 
-Lemma hvc_mem_retrieve_donate {E i wi sacc r0 sh j wf mem_rx p_rx} {ps: gset PID} ai wh:
+Lemma mem_retrieve_donate {E i wi sacc r0 sh j mem_rx p_rx} {ps: gset PID} ai wh:
   (* has access to the page which the instruction is in *)
   (tpa ai) ∈ sacc ->
   (* the current instruction is hvc *)
@@ -25,7 +25,7 @@ Lemma hvc_mem_retrieve_donate {E i wi sacc r0 sh j wf mem_rx p_rx} {ps: gset PID
        ▷ ([∗ set] p ∈ ps, p -@O> j) ∗
        ▷ i -@A> sacc ∗
        (* the transaction hasn't been retrieved *)
-       ▷ wh ->re false ∗ ▷ wh -{1}>t (j, wf, i, ps, Donation) ∗
+       ▷ wh ->re false ∗ ▷ wh -{1}>t (j, i, ps, Donation) ∗
        (* the rx page and locations that the rx descriptor will be at *)
        ▷ RX@ i := p_rx ∗ ▷ RX_state@ i := None ∗
        ▷ memory_page p_rx mem_rx ∗
@@ -45,14 +45,14 @@ Lemma hvc_mem_retrieve_donate {E i wi sacc r0 sh j wf mem_rx p_rx} {ps: gset PID
        RX@ i := p_rx ∗
        (∃ l des, RX_state@ i := Some(l, i) ∗ ⌜((Z.to_nat (finz.to_z l)) = (length des))%nat⌝ ∗
        (* XXX: not sure if it is useful *)
-       (⌜des = ([of_imm (encode_vmid j); wf; wh; encode_transaction_type Donation ;(l ^- 5)%f] ++ map of_pid (elements ps))⌝ ∗
+       (⌜des = ([of_imm (encode_vmid j); wh; encode_transaction_type Donation ;(l ^- 5)%f] ++ map of_pid (elements ps))⌝ ∗
                  memory_page p_rx ((list_to_map (zip (finz.seq p_rx (length des)) des)) ∪ mem_rx))) ∗
        (* the transaction is completed, deallocate it and release the handle *)
        fresh_handles 1 (sh ∪ {[wh]}) }}}.
 Proof.
 Admitted.
 
-Lemma hvc_mem_retrieve_donate_rx {E i wi sacc r0 sh j wf mem_rx } {ps: gset PID} ai wh:
+Lemma mem_retrieve_donate_rx {E i wi sacc r0 sh j mem_rx } {ps: gset PID} ai wh:
   (* the current instruction is hvc *)
   (* the decoding of wi is correct *)
   decode_instruction wi = Some(Hvc) ->
@@ -67,7 +67,7 @@ Lemma hvc_mem_retrieve_donate_rx {E i wi sacc r0 sh j wf mem_rx } {ps: gset PID}
        ▷ ([∗ set] p ∈ ps, p -@O> j) ∗
        ▷ i -@A> sacc ∗
        (* the transaction hasn't been retrieved *)
-       ▷ wh ->re false ∗ ▷ wh -{1}>t (j, wf, i, ps, Donation) ∗
+       ▷ wh ->re false ∗ ▷ wh -{1}>t (j, i, ps, Donation) ∗
        (* the rx page and locations that the rx descriptor will be at *)
        ▷ RX@ i := (tpa ai) ∗ ▷ RX_state@ i := None ∗
        ▷ (ai ->a wi -∗ memory_page (tpa ai) mem_rx) ∗
@@ -87,14 +87,14 @@ Lemma hvc_mem_retrieve_donate_rx {E i wi sacc r0 sh j wf mem_rx } {ps: gset PID}
        RX@ i := (tpa ai) ∗
        (∃ l des, RX_state@ i := Some(l, i) ∗ ⌜((Z.to_nat (finz.to_z l)) = (length des))%nat⌝ ∗
        (* XXX: not sure if it is useful *)
-       (⌜des = ([of_imm (encode_vmid j); wf; wh; encode_transaction_type Donation ;(l ^- 5)%f] ++ map of_pid (elements ps))⌝ ∗
+       (⌜des = ([of_imm (encode_vmid j); wh; encode_transaction_type Donation ;(l ^- 5)%f] ++ map of_pid (elements ps))⌝ ∗
                  memory_page (tpa ai) ((list_to_map (zip (finz.seq (tpa ai) (length des)) des)) ∪ mem_rx))) ∗
        (* the transaction is completed, deallocate it and release the handle *)
        fresh_handles 1 (sh ∪ {[wh]}) }}}.
 Proof.
 Admitted.
 
-Lemma hvc_mem_retrieve_invalid_handle {E i wi sacc r0 r2 wh} ai:
+Lemma mem_retrieve_invalid_handle {E i wi sacc r0 r2 wh} ai:
   (tpa ai) ∈ sacc ->
   (* the current instruction is hvc *)
   (* the decoding of wi is correct *)
@@ -121,7 +121,7 @@ Lemma hvc_mem_retrieve_invalid_handle {E i wi sacc r0 r2 wh} ai:
 Proof.
 Admitted.
 
-Lemma hvc_mem_retrieve_fresh_handle {E i wi sacc r0 r2 wh sh q} ai:
+Lemma mem_retrieve_fresh_handle {E i wi sacc r0 r2 wh sh q} ai:
   (tpa ai) ∈ sacc ->
   decode_instruction wi = Some(Hvc) ->
   decode_hvc_func r0 = Some(Retrieve) ->
@@ -144,7 +144,7 @@ Lemma hvc_mem_retrieve_fresh_handle {E i wi sacc r0 r2 wh sh q} ai:
 Proof.
 Admitted.
 
-Lemma hvc_mem_retrieve_invalid_trans {E i wi sacc r0 r2 wh meta q} ai:
+Lemma mem_retrieve_invalid_trans {E i wi sacc r0 r2 wh meta q} ai:
   (tpa ai) ∈ sacc ->
   decode_instruction wi = Some(Hvc) ->
   decode_hvc_func r0 = Some(Retrieve) ->
@@ -168,7 +168,7 @@ Lemma hvc_mem_retrieve_invalid_trans {E i wi sacc r0 r2 wh meta q} ai:
 Proof.
 Admitted.
 
-Lemma hvc_mem_retrieve_retrieved{E i wi sacc r0 r2 wh q} ai:
+Lemma mem_retrieve_retrieved{E i wi sacc r0 r2 wh q} ai:
   (tpa ai) ∈ sacc ->
   decode_instruction wi = Some(Hvc) ->
   decode_hvc_func r0 = Some(Retrieve) ->
@@ -191,7 +191,7 @@ Lemma hvc_mem_retrieve_retrieved{E i wi sacc r0 r2 wh q} ai:
 Proof.
 Admitted.
 
-Lemma hvc_mem_retrieve_rx_full{E i wi sacc r0 r2 q1 q2 j wf tt rx_state} {ps: gset PID} ai wh:
+Lemma mem_retrieve_rx_full{E i wi sacc r0 r2 q1 q2 j tt rx_state} {ps: gset PID} ai wh:
   (tpa ai) ∈ sacc ->
   decode_instruction wi = Some(Hvc) ->
   decode_hvc_func r0 = Some(Retrieve) ->
@@ -202,7 +202,7 @@ Lemma hvc_mem_retrieve_rx_full{E i wi sacc r0 r2 q1 q2 j wf tt rx_state} {ps: gs
        ▷ (R2 @@ i ->r r2) ∗
        ▷ i -@A> sacc ∗
        ▷ wh -{q1}>re false ∗
-       ▷ wh -{q2}>t (j,wf,i,ps,tt) ∗
+       ▷ wh -{q2}>t (j, i, ps, tt) ∗
        ▷ RX_state@i := rx_state
        }}}
    ExecI @ i; E
@@ -213,13 +213,13 @@ Lemma hvc_mem_retrieve_rx_full{E i wi sacc r0 r2 q1 q2 j wf tt rx_state} {ps: gs
        R2 @@ i ->r (encode_hvc_error Busy) ∗
        i -@A> sacc ∗
        wh -{q1}>re false ∗
-       wh -{q2}>t (j,wf,i,ps,tt) ∗
+       wh -{q2}>t (j, i, ps, tt) ∗
        RX_state@i := rx_state
    }}}.
 Proof.
 Admitted.
 
-Lemma hvc_mem_retrieve_lend{E i wi sacc r0 j wf mem_rx p_rx q} {ps: gset PID} ai wh:
+Lemma mem_retrieve_lend{E i wi sacc r0 j mem_rx p_rx q} {ps: gset PID} ai wh:
   (* has access to the page which the instruction is in *)
   (tpa ai) ∈ sacc ->
   (* the current instruction is hvc *)
@@ -235,7 +235,7 @@ Lemma hvc_mem_retrieve_lend{E i wi sacc r0 j wf mem_rx p_rx q} {ps: gset PID} ai
        (* the pagetable *)
        ▷ i -@A> sacc ∗
        (* the transaction hasn't been retrieved *)
-       ▷ wh ->re false ∗ ▷ wh -{q}>t (j, wf, i, ps, Lending) ∗
+       ▷ wh ->re false ∗ ▷ wh -{q}>t (j,  i, ps, Lending) ∗
        (* the rx page and locations that the rx descriptor will be at *)
        ▷ RX@ i := p_rx ∗ ▷ RX_state@ i := None ∗
        ▷ memory_page p_rx mem_rx}}}
@@ -248,18 +248,18 @@ Lemma hvc_mem_retrieve_lend{E i wi sacc r0 j wf mem_rx p_rx q} {ps: gset PID} ai
        R1 @@ i ->r wh ∗
        (* gain exclusive access and ownership *)
        i -@A> (ps ∪ sacc) ∗
-       wh ->re true ∗ wh -{q}>t (j, wf, i, ps, Lending) ∗
+       wh ->re true ∗ wh -{q}>t (j, i, ps, Lending) ∗
        (* new descriptor in rx *)
        RX@ i := p_rx ∗
        (∃ l des, RX_state@ i := Some(l, i) ∗ ⌜((Z.to_nat (finz.to_z l)) = (length des))%nat⌝ ∗
        (* XXX: not sure if it is useful *)
-       (⌜des = ([of_imm (encode_vmid j); wf; wh; encode_transaction_type Donation ;(l ^- 5)%f] ++ map of_pid (elements ps))⌝ ∗
+       (⌜des = ([of_imm (encode_vmid j); wh; encode_transaction_type Donation ;(l ^- 5)%f] ++ map of_pid (elements ps))⌝ ∗
                  memory_page p_rx ((list_to_map (zip (finz.seq p_rx (length des)) des)) ∪ mem_rx)))
         }}}.
 Proof.
 Admitted.
 
-Lemma hvc_mem_retrieve_lend_rx{E i wi sacc r0 j wf mem_rx q} {ps: gset PID} ai wh:
+Lemma mem_retrieve_lend_rx{E i wi sacc r0 j mem_rx q} {ps: gset PID} ai wh:
   (* the current instruction is hvc *)
   (* the decoding of wi is correct *)
   decode_instruction wi = Some(Hvc) ->
@@ -274,7 +274,7 @@ Lemma hvc_mem_retrieve_lend_rx{E i wi sacc r0 j wf mem_rx q} {ps: gset PID} ai w
        (* the pagetable *)
        ▷ i -@A> sacc ∗
        (* the transaction hasn't been retrieved *)
-       ▷ wh ->re false ∗ ▷ wh -{q}>t (j, wf, i, ps, Lending) ∗
+       ▷ wh ->re false ∗ ▷ wh -{q}>t (j, i, ps, Lending) ∗
        (* the rx page and locations that the rx descriptor will be at *)
        ▷ RX@ i := (tpa ai) ∗ ▷ RX_state@ i := None ∗
        ▷ (ai ->a wi -∗ memory_page (tpa ai) mem_rx)}}}
@@ -287,19 +287,19 @@ Lemma hvc_mem_retrieve_lend_rx{E i wi sacc r0 j wf mem_rx q} {ps: gset PID} ai w
        R1 @@ i ->r wh ∗
        (* gain exclusive access and ownership *)
        i -@A> (ps ∪ sacc) ∗
-       wh ->re true ∗ wh -{q}>t (j, wf, i, ps, Lending) ∗
+       wh ->re true ∗ wh -{q}>t (j, i, ps, Lending) ∗
        (* new descriptor in rx *)
        RX@ i := (tpa ai) ∗
        (∃ l des, RX_state@ i := Some(l, i) ∗ ⌜((Z.to_nat (finz.to_z l)) = (length des))%nat⌝ ∗
        (* XXX: not sure if it is useful *)
-       (⌜des = ([of_imm (encode_vmid j); wf; wh; encode_transaction_type Donation ;(l ^- 5)%f] ++ map of_pid (elements ps))⌝ ∗
+       (⌜des = ([of_imm (encode_vmid j); wh; encode_transaction_type Donation ;(l ^- 5)%f] ++ map of_pid (elements ps))⌝ ∗
                  memory_page (tpa ai) ((list_to_map (zip (finz.seq (tpa ai) (length des)) des)) ∪ mem_rx)))
         }}}.
 Proof.
 Admitted.
 
 
-Lemma hvc_mem_retrieve_share{E i wi sacc r0 j wf mem_rx p_rx q} {ps: gset PID} ai wh:
+Lemma mem_retrieve_share{E i wi sacc r0 j mem_rx p_rx q} {ps: gset PID} ai wh:
   (* has access to the page which the instruction is in *)
   (tpa ai) ∈ sacc ->
   (* the current instruction is hvc *)
@@ -316,7 +316,7 @@ Lemma hvc_mem_retrieve_share{E i wi sacc r0 j wf mem_rx p_rx q} {ps: gset PID} a
        (* the pagetable *)
        ▷ i -@A> sacc ∗
        (* the transaction hasn't been retrieved *)
-       ▷ wh ->re false ∗ ▷ wh -{q}>t (j, wf, i, ps, Sharing) ∗
+       ▷ wh ->re false ∗ ▷ wh -{q}>t (j, i, ps, Sharing) ∗
        (* the rx page and locations that the rx descriptor will be at *)
        ▷ RX@ i := p_rx ∗ ▷ RX_state@ i := None ∗
        ▷ memory_page p_rx mem_rx}}}
@@ -329,18 +329,18 @@ Lemma hvc_mem_retrieve_share{E i wi sacc r0 j wf mem_rx p_rx q} {ps: gset PID} a
        R1 @@ i ->r wh ∗
        (* gain exclusive access and ownership *)
        i -@A> (ps ∪ sacc) ∗
-       wh ->re true ∗ wh -{q}>t (j, wf, i, ps, Sharing) ∗
+       wh ->re true ∗ wh -{q}>t (j, i, ps, Sharing) ∗
        (* new descriptor in rx *)
        RX@ i := p_rx ∗
        (∃ l des, RX_state@ i := Some(l, i) ∗ ⌜((Z.to_nat (finz.to_z l)) = (length des))%nat⌝ ∗
        (* XXX: not sure if it is useful *)
-       (⌜des = ([of_imm (encode_vmid j); wf; wh; encode_transaction_type Donation ;(l ^- 5)%f] ++ map of_pid (elements ps))⌝ ∗
+       (⌜des = ([of_imm (encode_vmid j); wh; encode_transaction_type Donation ;(l ^- 5)%f] ++ map of_pid (elements ps))⌝ ∗
                  memory_page p_rx ((list_to_map (zip (finz.seq p_rx (length des)) des)) ∪ mem_rx)))
         }}}.
 Proof.
 Admitted.
 
-Lemma hvc_mem_retrieve_share_rx{E i wi sacc r0 j wf mem_rx q} {ps: gset PID} ai wh:
+Lemma mem_retrieve_share_rx{E i wi sacc r0 j mem_rx q} {ps: gset PID} ai wh:
   (* the current instruction is hvc *)
   (* the decoding of wi is correct *)
   decode_instruction wi = Some(Hvc) ->
@@ -355,7 +355,7 @@ Lemma hvc_mem_retrieve_share_rx{E i wi sacc r0 j wf mem_rx q} {ps: gset PID} ai 
        (* the pagetable *)
        ▷ i -@A> sacc ∗
        (* the transaction hasn't been retrieved *)
-       ▷ wh ->re false ∗ ▷ wh -{q}>t (j, wf, i, ps, Sharing) ∗
+       ▷ wh ->re false ∗ ▷ wh -{q}>t (j, i, ps, Sharing) ∗
        (* the rx page and locations that the rx descriptor will be at *)
        ▷ RX@ i := (tpa ai) ∗ ▷ RX_state@ i := None ∗
        ▷ (ai ->a wi -∗ memory_page (tpa ai) mem_rx)}}}
@@ -368,12 +368,12 @@ Lemma hvc_mem_retrieve_share_rx{E i wi sacc r0 j wf mem_rx q} {ps: gset PID} ai 
        R1 @@ i ->r wh ∗
        (* gain exclusive access and ownership *)
        i -@A> (ps ∪ sacc) ∗
-       wh ->re true ∗ wh -{q}>t (j, wf, i, ps, Sharing) ∗
+       wh ->re true ∗ wh -{q}>t (j, i, ps, Sharing) ∗
        (* new descriptor in rx *)
        RX@ i := (tpa ai) ∗
        (∃ l des, RX_state@ i := Some(l, i) ∗ ⌜((Z.to_nat (finz.to_z l)) = (length des))%nat⌝ ∗
        (* XXX: not sure if it is useful *)
-       (⌜des = ([of_imm (encode_vmid j); wf; wh; encode_transaction_type Donation ;(l ^- 5)%f] ++ map of_pid (elements ps))⌝ ∗
+       (⌜des = ([of_imm (encode_vmid j); wh; encode_transaction_type Donation ;(l ^- 5)%f] ++ map of_pid (elements ps))⌝ ∗
                  memory_page (tpa ai) ((list_to_map (zip (finz.seq (tpa ai) (length des)) des)) ∪ mem_rx)))
         }}}.
 Proof.
